src/SemBltn.v
@@ -1,0 +1,33 @@
+Require Import
+  Coq.ZArith.ZArith
+  Hask.Control.Monad
+  Hask.Data.Either
+  Pact.Bltn
+  Pact.SemTy
+  Pact.Lang.
+
+Set Implicit Arguments.
+Unset Strict Implicit.
+Unset Printing Implicit Defensive.
+
+Set Equations With UIP.
+
+Generalizable All Variables.
+Set Primitive Projections.
+
+Import ListNotations.
+
+Definition add : Z → Z → Z := Z.add.
+Definition sub : Z → Z → Z := Z.sub.
+
+Definition arity1 `(f : ty → ty') : ty → PactM ty' :=
+  λ n, pure (f n).
+
+Definition arity2 `(f : ty → ty' → ty'') : ty → PactM (ty' → PactM ty'') :=
+  λ n, pure (λ m, pure (f n m)).
+
+Definition SemBltn {τ} (bltn : Builtin τ) : SemTy τ :=
+  match bltn with
+  | AddInt => arity2 add
+  | SubInt => arity2 sub
+  end.
